theories/Term.v
@@ -7,133 +7,7 @@ Import IfNotations.
 
 Require Import FunInd.
 
-Instance multi_Reflexive: Reflexive multi.
-Proof using.
-  econstructor.
-Qed.
-
-Instance multi_trans: Transitive multi.
-Proof using.
-  intros v1 v2 v3 p.
-  generalize  v3.
-  induction p.
-  1: auto.
-  intros.
-  econstructor.
-  1: apply H.
-  apply IHp.
-  auto.
-Qed.
-
-Instance fst_Proper: Proper (step ==> step) v_fst.
-Proof.
-  intros ? ? p.
-  induction p.
-  all: constructor.
-  all: constructor.
-  all: auto.
-Defined.
-
-Instance snd_Proper: Proper (step ==> step) v_fst.
-Proof.
-  intros ? ? p.
-  induction p.
-  all: constructor.
-  all: constructor.
-  all: auto.
-Defined.
-
-Instance fanout_l_Proper x: Proper (step ==> step) (v_fanout x).
-Proof.
-  intros ? ? p.
-  induction p.
-  all: constructor.
-  all: constructor.
-  all: auto.
-Qed.
-
-Instance fanout_r_Proper: Proper (step ==> eq ==> step) v_fanout.
-Proof.
-  intros ? ? p.
-  induction p.
-  all: intros ? ? q.
-  all: subst.
-  all: constructor.
-  all: constructor.
-  all: auto.
-Defined.
-
-Instance fst_multi_Proper: Proper (multi ==> multi) v_fst.
-Proof.
-  intros ? ? p.
-  induction p.
-  1: reflexivity.
-  econstructor.
-  2: apply IHp.
-  constructor.
-  auto.
-Defined.
-
-Instance snd_multi_Proper: Proper (multi ==> multi) v_snd.
-Proof.
-  intros ? ? p.
-  induction p.
-  1: reflexivity.
-  econstructor.
-  2: apply IHp.
-  constructor.
-  auto.
-Defined.
-
-Instance fanout_multi_Proper: Proper (multi ==> multi ==> multi) v_fanout.
-Proof.
-  intros ? ? p.
-  induction p.
-  - intros ? ? q.
-    induction q.
-    + reflexivity.
-    + econstructor.
-      * eapply step_fanoutr.
-        eauto.
-      * auto.
-  - intros ? ? q.
-    induction q.
-    + econstructor.
-      2: eapply IHp.
-      1: econstructor.
-      1: auto.
-      reflexivity.
-    + econstructor.
-      2: apply IHq.
-      eapply step_fanoutr.
-      auto.
-Qed.
-
-Instance equiv_Reflexive: Reflexive Spec.equiv.
-Proof.
-  intros.
-  econstructor.
-  all: reflexivity.
-Defined.
-
-Instance equiv_Symmetric: Symmetric Spec.equiv.
-Proof.
-  intros ? ? [p q s].
-  exists s.
-  all: auto.
-Defined.
-
-(* FIXME seems like a big hole *)
-Instance equiv_Transitive: Transitive Spec.equiv.
-Proof.
-  admit.
-Admitted.
-
-Instance equiv_Equivalence: Equivalence Spec.equiv := { Equivalence_Reflexive := _ }.
-
-Instance term_Setoid: Setoid term := { equiv := Spec.equiv }.
-
-  Function typecheck (v: term): option type :=
+Function typecheck (v: term): option type :=
   match v with
   | v_tt => Some t_unit
   | v_fst v =>
@@ -191,7 +65,8 @@ Proof using .
   all: reflexivity.
 Qed.
 
-Definition of_t t := { v | ⊢ v in t }.
+Inductive tr A: Prop := tr_intro (_: A).
+Definition of_t t := { v | tr (⊢ v in t) }.
 
 Definition tc v: if typecheck v is Some t
                  then
@@ -202,83 +77,64 @@ Proof.
   destruct (typecheck v) eqn:q.
   2: apply tt.
   exists v.
+  exists.
   apply typecheck_sound.
   auto.
 Defined.
 
-Function beta v :=
+Function big v :=
   match v with
-  | v_fst (v_fanout v _) => Some v
-  | v_snd (v_fanout _ v) => Some v
-
-  | v_tt => None
-  | _ => None
-  end.
-
-Lemma beta_sound:
-  forall v v', beta v = Some v' -> Spec.beta v v'.
-Proof using.
-  intros v.
-  functional induction (beta v).
-  all: intros ? p.
-  all: inversion p.
-  all: constructor.
-Qed.
-
-Lemma beta_complete:
-  forall v v', Spec.beta v v' -> beta v = Some v'.
-Proof using.
-  intros ? ? p.
-  induction p.
-  all: reflexivity.
-Qed.
-
-Function eval v :=
-  match v with
-  | v_fst v => if eval v is Some v' then Some (v_fst v') else None
-  | v_snd v => if eval v is Some v' then Some (v_snd v') else None
+  | v_tt => Some v_tt
+  | v_fst v => if big v is Some (v_fanout a _) then Some a else None
+  | v_snd v => if big v is Some (v_fanout _ a) then Some a else None
   | v_fanout v0 v1 =>
-      if eval v0 is Some v0'
+      if big v0 is Some v0'
       then
-        Some (v_fanout v0' v1)
+        if big v1 is Some v1'
+        then
+          Some (v_fanout v0' v1')
+        else
+          None
       else
-          if eval v1 is Some v1'
-          then
-            Some (v_fanout v0 v1')
-          else
-            None
-  | _ => beta v
+        None
   end.
 
-Lemma beta_normal:
-  forall v, is_term_norm_of_term v = true -> beta v = None.
-Proof.
-  intros v.
-  functional induction (beta v).
-  all: cbn.
-  all: intros p.
-  all: inversion p.
-  all: reflexivity.
-Qed.
-
-Theorem eval_sound:
-  forall v v', eval v = Some v' -> v ~> v'.
+Theorem big_sound:
+  forall v v', big v = Some v' -> v ⇓ v'.
 Proof using.
   intros v.
-  functional induction (eval v).
-  all: cbn.
+  functional induction (big v).
   all: intros ? p.
   all: inversion p.
   all: subst.
-  all: econstructor.
-  all: eauto.
-  apply beta_sound.
-  auto.
+  - constructor.
+  - econstructor.
+    apply IHo.
+    eauto.
+  - econstructor.
+    apply IHo.
+    eauto.
+  - econstructor.
+    1: apply IHo.
+    2: apply IHo0.
+    all:  eauto.
 Qed.
 
-Theorem beta_preserve:
+Theorem big_complete:
+  forall v v', v ⇓ v' -> big v = Some v'.
+Proof using.
+  intros ? ? p.
+  induction p.
+  all: cbn.
+  all: try rewrite IHp.
+  all: try rewrite IHp1.
+  all: try rewrite IHp2.
+  all: reflexivity.
+Qed.
+
+Theorem big_preserve:
   forall v v',
-    Spec.beta v v' ->
+    v ⇓ v' ->
     forall t, ⊢ v in t -> ⊢ v' in t.
 Proof using.
   intros v v' p.
@@ -286,173 +142,75 @@ Proof using.
   all: intros ? q.
   all: inversion q.
   all: subst.
-  - inversion H0.
+  all: auto.
+  - econstructor.
+    all: eauto.
+  - set (p' := IHp _ H0).
+    inversion p'.
     subst.
     auto.
-  - inversion H0.
+  - set (p' := IHp _ H0).
+    inversion p'.
     subst.
     auto.
 Qed.
 
-Theorem step_preserve:
+Theorem big_normal:
   forall v v',
-    v ~> v' ->
-    forall t, ⊢ v in t -> ⊢ v' in t.
-Proof using.
-  intros v v' p.
-  induction p.
-  all: intros ? q.
-  - inversion q.
-    subst.
-    econstructor.
-    eauto.
-  - inversion q.
-    subst.
-    econstructor.
-    eauto.
-  - inversion q.
-    subst.
-    econstructor.
-    all: eauto.
-  - inversion q.
-    subst.
-    econstructor.
-    all: eauto.
-  - eapply beta_preserve.
-    all: eauto.
-Qed.
-
-Lemma multi_preserve:
-  forall v v',
-    v *~> v' ->
-    forall t, ⊢ v in t -> ⊢ v' in t.
-Proof using.
-  intros v v' p.
-  induction p.
-  1: auto.
-  intros t q.
-  apply IHp.
-  refine (step_preserve _ _ _ _ q).
-  auto.
-Qed.
-
-Theorem step_progress:
-  forall v t,
-    ⊢ v in t ->
-    is_term_norm_of_term v = false -> exists v', v ~> v'.
-Proof using.
-  intros v t p.
+    v ⇓ v' -> is_term_norm_of_term v' = true.
+Proof.
+  intros ? ? p.
   induction p.
   all: cbn.
-  all: intros q.
-  all: try discriminate.
-  - destruct (is_term_norm_of_term v1) eqn:q1,
-        (is_term_norm_of_term v2) eqn:q2.
-    all: try discriminate.
-    + destruct (IHp2 (eq_refl _)) as [v2' s2].
-      exists (v_fanout v1 v2').
-      constructor.
-      auto.
-    + destruct (IHp1 (eq_refl _)) as [v1' s1].
-      exists (v_fanout v1' v2).
-      constructor.
-      auto.
-    + destruct (IHp1 (eq_refl _)) as [v1' s1].
-      exists (v_fanout v1' v2).
-      constructor.
-      auto.
-  - destruct v.
-    all: cbn in IHp.
-    all: inversion p.
-    all: subst.
-    + destruct (IHp (eq_refl _)) as [v' s].
-      exists (v_fst v').
-      constructor.
-      auto.
-    + destruct (IHp (eq_refl _)) as [v' s].
-      exists (v_fst v').
-      constructor.
-      auto.
-    + exists v1.
-      econstructor.
-      constructor.
-  - destruct v.
-    all: cbn in IHp.
-    all: inversion p.
-    all: subst.
-    + destruct (IHp (eq_refl _)) as [v' s].
-      exists (v_snd v').
-      constructor.
-      auto.
-    + destruct (IHp (eq_refl _)) as [v' s].
-      exists (v_snd v').
-      constructor.
-      auto.
-    + exists v2.
-      econstructor.
-      constructor.
+  - reflexivity.
+  - rewrite IHp1, IHp2.
+    reflexivity.
+  - cbn in IHp.
+    destruct (is_term_norm_of_term N1).
+    1: reflexivity.
+    discriminate.
+  - cbn in IHp.
+    destruct (is_term_norm_of_term N1), (is_term_norm_of_term N2).
+    all: try reflexivity.
+    all: discriminate.
 Qed.
 
-Theorem multi_normalizing:
+Theorem normalize:
   forall v t,
-    ⊢ v in t ->
-   exists v', (v *~> v') /\ is_term_norm_of_term v' = true .
+   ⊢ v in t ->
+   { v' & v ⇓ v' }.
 Proof using.
-  intros v t p.
+  intros ? ? p.
   induction p.
   - exists v_tt.
-    split.
-    all: reflexivity.
-  - destruct IHp1 as [v1' [s1 n1]].
-    destruct IHp2 as [v2' [s2 n2]].
+    constructor.
+  - destruct IHp1 as [v1' s1].
+    destruct IHp2 as [v2' s2].
     exists (v_fanout v1' v2').
-    split.
-    + rewrite s1, s2.
-      reflexivity.
-    + cbn.
-      rewrite n1, n2.
-      cbn.
-      reflexivity.
-  - destruct IHp as [v' [s n]].
+    constructor.
+    all: auto.
+  - destruct IHp as [v' s].
+    set (vwf := big_preserve _ _ s _ p).
+    set (isnorm := big_normal _ _ s).
     destruct v'.
     all: cbn in *.
     all: try discriminate.
-    + set (p1 := multi_preserve _ _ s _ p).
-      inversion p1.
-    + set (p1 := multi_preserve _ _ s _ p).
-      inversion p1.
-      subst.
-      exists v'1.
-      split.
-      * rewrite s.
-        cbn.
-        econstructor.
-        2: reflexivity.
-        econstructor.
-        econstructor.
-      * destruct (is_term_norm_of_term v'1) eqn:q2.
-        2: discriminate.
-        reflexivity.
-  - destruct IHp as [v' [s n]].
+    all: inversion vwf.
+    all: subst.
+    all: cbn in *.
+    exists v'1.
+    econstructor.
+    all: eauto.
+  - destruct IHp as [v' s].
+    set (vwf := big_preserve _ _ s _ p).
+    set (isnorm := big_normal _ _ s).
     destruct v'.
     all: cbn in *.
     all: try discriminate.
-    + set (p1 := multi_preserve _ _ s _ p).
-      inversion p1.
-    + set (p1 := multi_preserve _ _ s _ p).
-      inversion p1.
-      subst.
-      exists v'2.
-      split.
-      * rewrite s.
-        cbn.
-        econstructor.
-        2: reflexivity.
-        econstructor.
-        econstructor.
-      * destruct (is_term_norm_of_term v'1) eqn:q1.
-        2: discriminate.
-        destruct (is_term_norm_of_term v'2) eqn:q2.
-        2: discriminate.
-        reflexivity.
+    all: inversion vwf.
+    all: subst.
+    all: cbn in *.
+    exists v'2.
+    econstructor.
+    all: eauto.
 Qed.
